Update example checksum log to use hashmap instead of hash_inv - somehow need to pass recover procedure the same hashmap from the crash predicate...?

src/ExampleChecksumLog.v
@@ -19,18 +19,18 @@ Definition hash_block : addr := $2.
 
 (* Representations for an example with two log blocks. *)
 (* block1 and block2 are synced, hash_block has some valid hash *)
-Definition any_hash_rep (a b a' b' : valu) (d : @mem addr (@weq addrlen) valuset) :
+Definition any_hash_rep (a b a' b' : valu) (d : @mem addr (@weq addrlen) valuset) hm :
     @pred addr (@weq addrlen) valuset :=
   (exists hv,
     [[ (block1 |-> (a, nil) *
      block2 |-> (b, nil) *
      hash_block |-> (hash_to_valu hv, nil))%pred d ]] *
-    [[ hash_list_rep (b' :: a' :: nil) hv ]])%pred.
+    [[ hash_list_rep (b' :: a' :: nil) hv hm ]])%pred.
 
 (* hash_block has the valid hash of block1 and block2 values *)
-Definition rep a b (d : @mem addr (@weq addrlen) valuset) :
+Definition rep a b (d : @mem addr (@weq addrlen) valuset) hm :
     @pred addr (@weq addrlen) valuset :=
-  any_hash_rep a b a b d.
+  any_hash_rep a b a b d hm.
 
 (* After a crash:
   - block1 and block2 can be anything
@@ -38,95 +38,96 @@ Definition rep a b (d : @mem addr (@weq addrlen) valuset) :
     - hash of old values
     - hash of new values but unsynced
     - hash of new values and synced *)
-Definition crep (a b a' b' : valu) :
+Definition crep (a b a' b' : valu) hm :
     @pred addr (@weq addrlen) valuset :=
   (exists hv hv',
     block1 |->? *
     block2 |->? *
     ( hash_block |-> (hash_to_valu hv, nil) *
-        [[ hash_list_rep (b :: a :: nil) hv ]] \/
+        [[ hash_list_rep (b :: a :: nil) hv hm ]] \/
       hash_block |-> (hash_to_valu hv', hash_to_valu hv :: nil) *
-        [[ hash_list_rep (b :: a :: nil) hv /\ hash_list_rep (b' :: a' :: nil) hv' ]] \/
+        [[ hash_list_rep (b :: a :: nil) hv hm /\ hash_list_rep (b' :: a' :: nil) hv' hm ]] \/
       hash_block |-> (hash_to_valu hv', nil) *
-        [[ hash_list_rep (b' :: a' :: nil) hv' ]]))%pred.
+        [[ hash_list_rep (b' :: a' :: nil) hv' hm ]]))%pred.
 
 
 (* Example "log" implementation using checksums *)
-Definition put T cs d1 d2 rx : prog T :=
+Definition put T cs hm d1 d2 rx : prog T :=
   cs <- BUFCACHE.write block1 d1 cs;
   cs <- BUFCACHE.write block2 d2 cs;
-  h <- hash_list (d1 :: d2 :: nil);
+  let^ (h, hm) <- hash_list (d1 :: d2 :: nil) hm;
   cs <- BUFCACHE.write hash_block (hash_to_valu h) cs;
   cs <- BUFCACHE.sync block1 cs;
   cs <- BUFCACHE.sync block2 cs;
   cs <- BUFCACHE.sync hash_block cs;
-  rx cs.
+  rx ^(cs, hm).
 
-Definition get T cs rx : prog T :=
+Definition get T cs (hm : hashmap) rx : prog T :=
   let^ (cs, d1) <- BUFCACHE.read block1 cs;
   let^ (cs, d2) <- BUFCACHE.read block2 cs;
   rx ^(d1, d2).
 
-Definition recover T cs rx : prog T :=
+Definition recover T cs hm rx : prog T :=
   let^ (cs, d1) <- BUFCACHE.read block1 cs;
   let^ (cs, d2) <- BUFCACHE.read block2 cs;
   let^ (cs, diskh) <- BUFCACHE.read hash_block cs;
-  h <- hash_list (d1 :: d2 :: nil);
+  let^ (h, hm) <- hash_list (d1 :: d2 :: nil) hm;
   If (weq diskh (hash_to_valu h)) {
-    rx cs
+    rx ^(cs, hm)
   } else {
-    cs <- put cs default_valu default_valu;
-    rx cs
+    let^ (cs, hm) <- put cs hm default_valu default_valu;
+    rx ^(cs, hm)
   }.
 
 
-Theorem put_ok : forall cs d1 d2,
+Theorem put_ok : forall cs d1 d2 hm,
   {< d d1_old d2_old d1_old' d2_old',
   PRE
     BUFCACHE.rep cs d *
-    any_hash_rep d1_old d2_old d1_old' d2_old' d
-  POST RET:cs'
+    any_hash_rep d1_old d2_old d1_old' d2_old' d hm
+  POST RET:^(cs', hm')
     exists d',
       BUFCACHE.rep cs' d' *
-      rep d1 d2 d'
+      rep d1 d2 d' hm'
   CRASH
-    exists cs' d',
+    exists cs' d' hm',
       BUFCACHE.rep cs' d' *
-      [[ (crep d1_old' d2_old' d1 d2)%pred d' ]]
-  >} put cs d1 d2.
+      [[ (crep d1_old' d2_old' d1 d2 hm')%pred d' ]]
+  >} put cs hm d1 d2.
 Proof.
   unfold put, rep, any_hash_rep, crep.
   step.
   step.
   step.
   apply goodSize_bound with (bound := 2); auto.
-  step.
+  step;
+  eapply hash_list_rep_subset in H as H'; eauto.
   step.
   step.
   step.
   step.
 
-  all: cancel.
+  all: cancel_with eauto.
   Grab Existential Variables.
   all: eauto.
 Qed.
 
-Hint Extern 1 ({{_}} progseq (put _ _ _) _) => apply put_ok : prog.
+Hint Extern 1 ({{_}} progseq (put _ _ _ _) _) => apply put_ok : prog.
 
 
-Theorem get_ok : forall cs,
+Theorem get_ok : forall cs hm,
   {< d d1 d2,
   PRE
     BUFCACHE.rep cs d *
-    rep d1 d2 d
+    rep d1 d2 d hm
   POST RET:^(d1', d2')
     exists cs', BUFCACHE.rep cs' d *
-    rep d1 d2 d *
+    rep d1 d2 d hm *
     [[ d1 = d1' /\ d2 = d2' ]]
   CRASH
     exists cs', BUFCACHE.rep cs' d *
-    rep d1 d2 d
-  >} get cs.
+    rep d1 d2 d hm
+  >} get cs hm.
 Proof.
   unfold get, rep, any_hash_rep.
   step.
@@ -135,18 +136,18 @@ Proof.
 Qed.
 
 (* block1 and block2 get some value, and hash_block points to a valid hash of  *)
-Definition after_crash_pred (v1 v2 : valu) :
+Definition after_crash_pred (v1 v2 : valu) hm :
     @pred addr (@weq addrlen) valuset :=
   (exists a b hv,
       block1 |-> (a, nil) *
       block2 |-> (b, nil) *
       hash_block |-> (hash_to_valu hv, nil) *
-    [[ hash_list_rep (v2 :: v1 :: nil) hv ]])%pred.
+    [[ hash_list_rep (v2 :: v1 :: nil) hv hm ]])%pred.
 
-Lemma crash_xform_would_recover_either_pred : forall v1 v2 v1' v2',
-  crash_xform (crep v1 v2 v1' v2') =p=>
-    after_crash_pred v1 v2 \/
-    after_crash_pred v1' v2'.
+Lemma crash_xform_would_recover_either_pred : forall v1 v2 v1' v2' hm,
+  crash_xform (crep v1 v2 v1' v2' hm) =p=>
+    after_crash_pred v1 v2 hm \/
+    after_crash_pred v1' v2' hm.
 Proof.
   unfold crep, after_crash_pred.
   intros.
@@ -156,25 +157,25 @@ Qed.
 Hint Rewrite crash_xform_would_recover_either_pred : crash_xform.
 
 
-Theorem recover_ok : forall cs,
+Theorem recover_ok : forall cs hm,
   {< d1_old d2_old d1 d2,
   PRE
     exists d,
       BUFCACHE.rep cs d *
-      [[ crash_xform (crep d1_old d2_old d1 d2)%pred d ]]
-  POST RET:cs'
+      [[ crash_xform (crep d1_old d2_old d1 d2 hm)%pred d ]]
+  POST RET:^(cs', hm')
     exists d',
       BUFCACHE.rep cs' d' *
-      (rep d1_old d2_old d' \/
-       rep d1 d2 d' \/
-       rep default_valu default_valu d')
+      (rep d1_old d2_old d' hm' \/
+       rep d1 d2 d' hm' \/
+       rep default_valu default_valu d' hm')
   CRASH
-    exists cs' d',
+    exists cs' d' hm',
       (BUFCACHE.rep cs' d' *
-       [[ (crep d1_old d2_old default_valu default_valu)%pred d' ]]) \/
+       [[ (crep d1_old d2_old default_valu default_valu hm')%pred d' ]]) \/
       (BUFCACHE.rep cs' d' *
-       [[ (crep d1 d2 default_valu default_valu)%pred d' ]])
-  >} recover cs.
+       [[ (crep d1 d2 default_valu default_valu hm')%pred d' ]])
+  >} recover cs hm.
 Proof.
   unfold recover, rep.
   intros.
@@ -182,8 +183,8 @@ Proof.
   intros. norm'l. unfold stars; simpl.
 
   (* autorewrite with crash_xform doesn't work? *)
-  assert (Hafter_crash: (after_crash_pred d1_old d2_old)%pred d \/
-    (after_crash_pred d1 d2)%pred d).
+  assert (Hafter_crash: (after_crash_pred d1_old d2_old hm)%pred d \/
+    (after_crash_pred d1 d2 hm)%pred d).
     apply crash_xform_would_recover_either_pred.
     auto.
 
@@ -198,23 +199,25 @@ Proof.
     apply goodSize_bound with (bound := 2); auto.
     step.
     step.
-    apply hash_to_valu_inj in H8.
+    apply hash_to_valu_inj in H9.
     subst.
     assert (Hheq: d1_old = a /\ d2_old = b).
-      eapply hash_list_injective in H5; try apply H10.
-      inversion H5. auto.
+      eapply hash_list_rep_subset in H0; eauto.
+      eapply hash_list_injective in H0; try apply H11.
+      inversion H0. auto.
     unfold any_hash_rep.
     cancel_with eauto.
 
     step.
     unfold any_hash_rep.
     cancel_with eauto.
+    eapply hash_list_rep_subset; eauto.
     step.
     all: repeat cancel; try (
       unfold crep in *;
       instantiate (1:=d);
       apply pimpl_or_r; left;
-      repeat cancel).
+      repeat cancel_with eauto).
 
   - cancel.
     step.
@@ -223,23 +226,25 @@ Proof.
     apply goodSize_bound with (bound := 2); auto.
     step.
     step.
-    apply hash_to_valu_inj in H8.
+    apply hash_to_valu_inj in H9.
     subst.
     assert (Hheq: d1 = a /\ d2 = b).
-      eapply hash_list_injective in H5; try apply H10.
-      inversion H5. auto.
+      eapply hash_list_rep_subset in H0; eauto.
+      eapply hash_list_injective in H0; try apply H11.
+      inversion H0. auto.
     unfold any_hash_rep.
     cancel_with eauto.
 
     step.
     unfold any_hash_rep.
     cancel_with eauto.
+    eapply hash_list_rep_subset; eauto.
     step.
     all: repeat cancel; try (
       unfold crep in *;
       instantiate (1:=d);
       apply pimpl_or_r; right;
-      repeat cancel).
+      repeat cancel_with eauto).
 
   Grab Existential Variables.
   all: eauto.
